---
title: Ackermann_function
permalink: Ackermann_function
---

The Ackermann function, expressed as \\(A(a,b)\\), is a function for expressing extremely large numbers.

## Defination
The Ackermann function is defined as follows:

\\(A(0,b)=b+1 \\\\ A(a,0)=A(a-1,1) \\\\ A(a,b)=A(a-1,A(a,b-1))\\)

## Example
\\begin{eqnarray*} A(4,3) &=&
A(3,A(4,2)) \\\\ &=&
A(3,A(3,A(4,1))) \\\\ &=&
A(3,A(3,A(3,A(4,0)))) \\\\ &=&
A(3,A(3,A(3,A(3,1)))) \\\\ &=&
A(3,A(3,A(3,A(2,A(3,0))))) \\\\ &=&
A(3,A(3,A(3,A(2,A(2,1))))) \\\\ &=&
A(3,A(3,A(3,A(2,A(1,A(2,0)))))) \\\\ &=&
A(3,A(3,A(3,A(2,A(1,A(1,1)))))) \\\\ &=&
A(3,A(3,A(3,A(2,A(1,A(0,A(1,0))))))) \\\\ &=&
A(3,A(3,A(3,A(2,A(1,A(0,A(0,1))))))) \\\\ &=&
A(3,A(3,A(3,A(2,A(1,A(0,2)))))) \\\\ &=&
A(3,A(3,A(3,A(2,A(1,3))))) \\\\ &=&
A(3,A(3,A(3,A(2,A(0,A(1,2)))))) \\\\ &=&
A(3,A(3,A(3,A(2,A(0,A(0,A(1,1))))))) \\\\ &=&
A(3,A(3,A(3,A(2,A(0,A(0,A(0,A(1,0)))))))) \\\\ &=&
A(3,A(3,A(3,A(2,A(0,A(0,A(0,A(0,1)))))))) \\\\ &=&
A(3,A(3,A(3,A(2,A(0,A(0,A(0,2))))))) \\\\ &=&
A(3,A(3,A(3,A(2,A(0,A(0,3)))))) \\\\ &=&
A(3,A(3,A(3,A(2,A(0,4))))) \\\\ &=&
A(3,A(3,A(3,A(2,5)))) \\end{eqnarray*}

## Explicit formula
We now prove that \\(A(a,b)=2\\uparrow^{a-2}(b+3)-3\\) for \\(a>2\\).

\\[A(0,b)=b+1 \\\\ A(1,b)=A(0,A(1,b-1))=A(1,b-1)+1=A(1,b-2)+2=\\cdots=A(1,b-b)+b=b+2 \\\\ A(2,b)=A(1,A(2,b-1))=A(2,b-1)+2\\times1=A(2,b-2)+2\\times2=\\cdots=A(2,b-b)+2b=2b+3=2(b+3)-3 \\\\ A(3,b)=A(2,A(3,b-1))=2(A(3,b-1)+3)-3=2^2(A(3,b-2)+3)-3=\\cdots=2^b(A(3,0)+3)-3=2^{b+3}-3\\]

Assuming that this holds true for \\(a=k\\), for \\(a=k+1\\):

\\[A(k+1,b)=A(k,A(k+1,b-1))=2\\uparrow^{k-2}(A(k,A(k+1,b-2)+3)-3=\\cdots=\\underbrace{2\\uparrow^{k-2}2\\uparrow^{k-2}\\cdots\\uparrow^{k-2}(A(k+1,0)+3)}\_{\\text{b 2's}}-3=\\underbrace{2\\uparrow^{k-2}2\\uparrow^{k-2}\\cdots\\uparrow^{k-2}2\\uparrow^{k-2}2}\_{\\text{b+3 2's}}-3=2\\uparrow^{k-1}(b+3)-3\\]

QED.