---
title: Bird%27s_array_notation
permalink: Bird%27s_array_notation
---

Bird's array notation is a parallel notation to [BEAF](BEAF "BEAF").

# Linear arrays

-   **Rule 1**. With one or two entries, we have $\\{a\\} = a$, $\\{a,b\\} = a^b$.
-   **Rule 2**. If the last entry is 1, it can be removed: $\\{\\#,1\\} = \\{\\#\\}$.
-   **Rule 3**. If the second entry is 1, the value is just the first entry: $\\{a,1 \\#\\} = a$.
-   **Rule 4**. If the third entry is 1:
-   :$\\{a,b,\\underbrace{1,1,\\cdots,1,1}\_n,c \\#\\} = \\{\\underbrace{a,a,a,a,\\cdots,a}\_{n+1},\\{a,b-1,\\underbrace{1,1,\\cdots,1,1}\_n,c \\#\\},c-1 \\#\\}$
-   **Rule 5**. Otherwise:
-   :$\\{a,b,c \\#\\} = \\{a,\\{a,b-1,c \\#\\},c-1 \\#\\}$

Limit: $\\{n,n[2]2\\}$ has growth rate $\\omega^\\omega$

## Example

\\begin{eqnarray*} \\{3,3,1,2\\} &=& \\{3,3,\\{3,2,1,2\\},1\\} \\\\ &=&
\\{3,3,\\{3,3,\\{3,1,1,2\\},1\\}\\} \\\\ &=&
\\{3,3,\\{3,3,3\\}\\} \\\\ &=&
\\{3,3,\\{3,\\{3,2,3\\},2\\}\\} \\\\ &=&
\\{3,3,\\{3,\\{3,\\{3,1,3\\},2\\},2\\}\\} \\\\ &=&
\\{3,3,\\{3,\\{3,3,2\\},2\\}\\} \\\\ &=&
\\{3,3,\\{3,\\{3,\\{3,2,2\\},1\\},2\\}\\} \\\\ &=&
\\{3,3,\\{3,\\{3,\\{3,\\{3,1,2\\},1\\}\\},2\\}\\} \\\\ &=&
\\{3,3,\\{3,\\{3,\\{3,3\\}\\},2\\}\\} \\\\ &=&
\\{3,3,\\{3,7625597484987,2\\}\\} \\\\ &=&
3\\uparrow^{3\\uparrow\\uparrow7625597484987}3 \\end{eqnarray*}

# Multidimentional arrays

-   **Rule M1**. If there are only two entries, $\\{a, b\\} = a^b$.
-   **Rule M2**. If $m < n$, we have $\\{\\# [m] 1 [n] \\#^*\\} = \\{\\# [n] \\#^*\\}$. (This also removes ones from the end of an array.)
-   **Rule M3**. If the second entry is 1, we have $\\{a,1 \\#\\} = a$.
-   **Rule M4**. If there is a non-zero entry immediately after batch of unfilled separators:
-   :$\\{a,b [m\_1] 1 [m\_2] \\cdots 1 [m\_x] c \\#\\} = \\{a \\langle m\_1-1 \\rangle b [m\_1] a \\langle m\_2-1 \\rangle b [m\_2] \\cdots a \\langle m\_x-1 \\rangle b [m\_x] (c-1) \\#\\}$
-   **Rule M5**. If there is a non-zero entry after batch of unfilled separators and a 1.
-   :$\\{a,b [m\_1] 1 [m\_2] \\cdots 1 [m\_x] 1,c \\#\\} = \\{a \\langle m\_1-1 \\rangle b [m\_1] a \\langle m\_2-1 \\rangle b [m\_2] \\cdots a \\langle m\_x-1 \\rangle b [m\_x] \\{a,b-1 [m\_1] 1 [m\_2] \\cdots 1 [m\_x] 1,c \\#\\},c-1 \\#\\}$
-   **Rule M6**. Rules M1-M5 don't apply.
-   :$\\{a,b,c \\#\\} = \\{a,\\{a,b-1,c \\#\\},c-1 \\#\\}$
-   **Rule A1**. If $c = 0$, we have $\\textrm\` a \\langle 0 \\rangle b = a \\textrm'$.
-   **Rule A2**. If $b = 1$, we have $\\textrm\` a \\langle c \\rangle 1 = a \\textrm'$.
-   **Rule A3**. Otherwise, $\\textrm\` a \\langle c \\rangle b \\textrm' = \\textrm\` \\underbrace{a \\langle c-1 \\rangle b [c] \\cdots [c] a \\langle c-1 \\rangle b}\_b \\textrm'$.

Limit: $\\{n,n[1,2]2\\}$ has growth rate $\\omega^{\\omega^\\omega}$

## Example

\\begin{eqnarray*} \\{3,2[3]2\\} &=& \\{3 \\langle 2 \\rangle 2[3]1\\} \\\\ &=&
\\{3 \\langle 1 \\rangle 2[2]3 \\langle 1 \\rangle 2\\} \\\\ &=&
\\{3,3[2]3,3\\} \\\\ &=&
\\{3,3,3[2]2,3\\} \\\\ &=&
\\{3,\\{3,2,3[2]2,3\\},2[2]2,3\\} \\\\ &=&
\\{3,\\{3,3,2[2]2,3\\},2[2]2,3\\} \\\\ &=&
\\{3,\\{3,\\{3,2,2[2]2,3\\}[2]2,3\\},2[2]2,3\\} \\\\ &=&
\\{3,\\{3,\\{3,3[2]2,3\\}[2]2,3\\},2[2]2,3\\} \\\\ &=&
\\{3,\\{3,\\{3,\\{3,\\{3,3[2]1,3\\}[2]1,3\\},2[2]1,3\\}[2]2,3\\},2[2]2,3\\}
\\end{eqnarray*}

# Hyperdimentional arrays

-   **Rule M1**. If there are only two entries, $\\{a, b\\} = a^b$.
-   **Rule M2**. If $m < n$, we have $\\{\\# [m] 1 [n] \\#^*\\} = \\{\\# [n] \\#^*\\}$. (This also removes ones from the end of an array.)
-   **Rule M3**. If the second entry is 1, we have $\\{a,1 \\#\\} = a$.
-   **Rule M4**. If there is a non-zero entry immediately after batch of unfilled separators:
-   :$\\{a,b [m\_1 \\#\_1] 1 [m\_2 \\#\_2] \\cdots 1 [m\_x \\#\_x] c \\#\\} = \\{a \\langle m\_1-1 \\#\_1 \\rangle b [m\_1 \\#\_1] a \\langle m\_2-1 \\#\_2 \\rangle b [m\_2 \\#\_2] \\cdots a \\langle m\_x-1 \\#\_x \\rangle b [m\_x \\#\_x] (c-1) \\#\\}$
-   **Rule M5**. If there is a non-zero entry after batch of unfilled separators and a 1.
-   :$\\{a,b [m\_1 \\#\_1] 1 [m\_2 \\#\_2] \\cdots 1 [m\_x \\#\_x] 1,c \\#\\}$<br />$= \\{a \\langle m\_1-1 \\#\_1 \\rangle b [m\_1 \\#\_1] a \\langle m\_2-1 \\#\_2 \\rangle b [m\_2 \\#\_2] \\cdots a \\langle m\_x-1 \\#\_x \\rangle b [m\_x \\#\_x] \\{a,b-1 [m\_1 \\#\_1] 1 [m\_2 \\#\_2] \\cdots 1 [m\_x \\#\_x] 1,c \\#\\},c-1 \\#\\}$
-   **Rule M6**. Rules M1-M5 don't apply.
-   :$\\{a,b,c \\#\\} = \\{a,\\{a,b-1,c \\#\\},c-1 \\#\\}$
-   **Rule A1**. If $c = 0$, we have $\\textrm\` a \\langle 0 \\rangle b = a \\textrm'$.
-   **Rule A2**. If $b = 1$, we have $\\textrm\` a \\langle A \\rangle 1 = a \\textrm'$.
-    **Rule A3**. If the first entry in the angle brackets is zero, and there exists a non-zero entry after it:
-   : $\\textrm\` a \\langle 0,\\underbrace{1,1,\\cdots,1,1}\_n,c \\# \\rangle b \\textrm' = \\textrm\` a \\langle \\underbrace{b,b,b,\\cdots,b,b}\_{n+1},c-1 \\# \\rangle b \\textrm'$
-   **Rule A4**. Otherwise, $\\textrm\` a \\langle c \\# \\rangle b \\textrm' = \\textrm\` \\underbrace{a \\langle c-1 \\# \\rangle b [c \\#] \\cdots [c \\#] a \\langle c-1 \\# \\rangle b}\_b \\textrm'$.

Limit: $\\{n,n[1[2]2]2\\}$ has growth rate $^4 \\omega$

## Example

\\begin{eqnarray*} \\{3,2[1,1,2]2\\} &=& \\{3 \\langle 0,1,2 \\rangle 2\\} \\\\ &=&
\\{3 \\langle 2,2 \\rangle 2\\} \\\\ &=&
\\{3 \\langle 1,2 \\rangle 2[2,2]3 \\langle 1,2 \\rangle 2\\} \\\\ &=&
\\{3,3[2]3,3[1,2]3,3[2]3,3[2,2]3,3[2]3,3[1,2]3,3[2]3,3\\}
\\end{eqnarray*}

# Nested arrays

Main rules will remain the same forever.

-   **Rule A1**. If $c = 0$, we have $\\textrm\` a \\langle 0 \\rangle b = a \\textrm'$.
-   **Rule A2**. If $b = 1$, we have $\\textrm\` a \\langle A \\rangle 1 = a \\textrm'$.
-   **Rule A3**. If $[A] < [B]$, $\\textrm\` a \\langle \\# [A] 1 [B] \\#^* \\rangle b \\textrm' = \\textrm\` a \\langle \\# [B] \\#^* \\rangle b \\textrm'$.
-   **Rule A4**. If the first entry in the angle brackets is zero, and there exists a non-zero entry after it:
-   : $\\textrm\` a \\langle 0 [x\_1 \\#\_1] 1 [x\_2 \\#\_2] \\cdots 1 [x\_n \\#\_n] c \\# \\rangle b \\textrm' = \\textrm\` a \\langle b \\langle x\_1-1 \\#\_1 \\rangle b [x\_1 \\#\_1] b \\langle x\_2-1 \\#\_2 \\rangle b [x\_2 \\#\_2] \\cdots b \\langle x\_n-1 \\#\_n \\rangle b [x\_n \\#\_n] c-1 \\# \\rangle b \\textrm'$
-   **Rule A5**. Otherwise, $\\textrm\` a \\langle c \\# \\rangle b \\textrm' = \\textrm\` \\underbrace{a \\langle c-1 \\# \\rangle b [c \\#] \\cdots [c \\#] a \\langle c-1 \\# \\rangle b}\_b \\textrm'$.

Limit: $\\{n,n[1\\backslash2]2\\}$ has growth rate $\\varepsilon\_0$

## Example

\\begin{eqnarray*} \\{3,2[1[2]2]2\\} &=& \\{3 \\langle 0[2]2 \\rangle 2\\} \\\\ &=&
\\{3 \\langle 2 \\langle 1 \\rangle 2 \\rangle 2\\} \\\\ &=&
\\{3 \\langle 2,2 \\rangle 2\\} \\\\ &=&
\\{3,3[2]3,3[1,2]3,3[2]3,3[2,2]3,3[2]3,3[1,2]3,3[2]3,3\\}
\\end{eqnarray*}

# Hyper-Nested arrays

-   **Rule A1**. If $c = 0$, we have $\\textrm\` a \\langle 0 \\rangle b \\textrm' = \\textrm\` a \\textrm'$ and $\\textrm\` a \\langle 0 \\rangle \\backslash b \\textrm'  = \\textrm\` a \\textrm'$.
-   **Rule A2**. If $b = 1$, we have $\\textrm\` a \\langle A \\rangle 1 \\textrm' = \\textrm\` a \\textrm'$ and $\\textrm\` a \\langle A \\rangle \\backslash 1 \\textrm' = \\textrm\` a \\textrm'$.
-   **Rule A3**. If $[A] < [B]$, $\\textrm\` a \\langle \\# [A] 1 [B] \\#^* \\rangle b \\textrm' = \\textrm\` a \\langle \\# [B] \\#^* \\rangle b \\textrm'$ and $\\textrm\` a \\langle \\# [A] 1 [B] \\#^* \\rangle \\backslash b \\textrm' = \\textrm\` a \\langle \\# [B] \\#^* \\rangle \\backslash b \\textrm'$.
-   **Rule A4**. If the first entry in the angle brackets is zero, and there exists a non-zero entry after it:
-   : $\\textrm\` a \\langle 0 [x\_1 \\#\_1]\\backslash 1 [x\_2 \\#\_2]\\backslash \\cdots 1 [x\_m \\#\_m]\\backslash 1 [y\_1 \\#^*\_1] 1 [y\_2 \\#^*\_2] \\cdots [y\_n \\#^*\_n] c \\# \\rangle b \\textrm'$<br />$= \\textrm\` a \\langle b \\langle x\_1-1 \\#\_1 \\rangle \\backslash b [x\_1 \\#\_1]\\backslash b \\langle x\_2-1 \\#\_2 \\rangle \\backslash b [x\_2 \\#\_2]\\backslash \\cdots b \\langle x\_n-1 \\#\_n \\rangle \\backslash b [x\_n \\#\_n]\\backslash b \\langle y\_1-1 \\#^*\_1 \\rangle b [y\_1 \\#^*\_1] b \\langle y\_2-1 \\#^*\_2 \\rangle b [y\_2 \\#^*\_2] \\cdots b \\langle y\_n-1 \\#^*\_n \\rangle b [y\_n \\#^*\_n] c-1 \\# \\rangle b \\textrm'$.
-   : $\\textrm\` a \\langle 0 [x\_1 \\#\_1]\\backslash 1 [x\_2 \\#\_2]\\backslash \\cdots 1 [x\_m \\#\_m]\\backslash 1 [y\_1 \\#^*\_1] 1 [y\_2 \\#^*\_2] \\cdots [y\_n \\#^*\_n] c \\# \\rangle \\backslash b \\textrm'$<br />$= \\textrm\` a \\langle b \\langle x\_1-1 \\#\_1 \\rangle \\backslash b [x\_1 \\#\_1]\\backslash b \\langle x\_2-1 \\#\_2 \\rangle \\backslash b [x\_2 \\#\_2]\\backslash \\cdots b \\langle x\_n-1 \\#\_n \\rangle \\backslash b [x\_n \\#\_n]\\backslash b \\langle y\_1-1 \\#^*\_1 \\rangle b [y\_1 \\#^*\_1] b \\langle y\_2-1 \\#^*\_2 \\rangle b [y\_2 \\#^*\_2] \\cdots b \\langle y\_n-1 \\#^*\_n \\rangle b [y\_n \\#^*\_n] c-1 \\# \\rangle \\backslash b \\textrm'$.
-   **Rule A5**. First non-zero entry is prior to a single backslash:
-   : $\\textrm\` a \\langle 0 [x\_1 \\#\_1]\\backslash 1 [x\_2 \\#\_2]\\backslash \\cdots 1 [x\_n \\#\_n]\\backslash 1 \\backslash c \\# \\rangle b\\textrm'$<br />$= \\textrm\`a \\langle b \\langle A\_1' \\rangle\\backslash b [A\_1]\\backslash b \\langle A\_2' \\rangle\\backslash b [A\_2]\\backslash \\cdots b \\langle A\_n' \\rangle\\backslash b [A\_n]\\backslash R\_b \\backslash c-1 \\# \\rangle b\\textrm'$;
-   : $\\textrm\` a \\langle 0 [x\_1 \\#\_1]\\backslash 1 [x\_2 \\#\_2]\\backslash \\cdots 1 [x\_n \\#\_n]\\backslash 1 \\backslash c \\# \\rangle \\backslash b\\textrm'$<br />$= \\textrm\`a \\langle b \\langle A\_1' \\rangle\\backslash b [A\_1]\\backslash b \\langle A\_2' \\rangle\\backslash b [A\_2]\\backslash \\cdots b \\langle A\_n' \\rangle\\backslash b [A\_n]\\backslash R\_b \\backslash c-1 \\# \\rangle \\backslash b\\textrm'$.
-   **Rule A6**. Otherwise, $\\textrm\` a \\langle c \\# \\rangle b \\textrm' = \\textrm\` \\underbrace{a \\langle c-1 \\# \\rangle b [c \\#] \\cdots [c \\#] a \\langle c-1 \\# \\rangle b}\_b \\textrm'$ and $\\textrm\` a \\langle c \\# \\rangle \\backslash b \\textrm' = \\textrm\` \\underbrace{a \\langle c-1 \\# \\rangle \\backslash b [c \\#]\\backslash \\cdots [c \\#]\\backslash a \\langle c-1 \\# \\rangle \\backslash b}\_b \\textrm'$.

Limit: $\\{n,n[1/2]2\\}$ has growth rate $\\Gamma\_0$.

## Examples

\\begin{eqnarray*} \\{3 \\langle 0 \\backslash 2 \\rangle 2\\} &=& \\{3 \\langle R\_2 \\rangle 2\\} \\\\ &=&
\\{3 \\langle 2 \\rangle 2\\} \\\\ &=&
\\{3,3[2]3,3\\} \\\\ &=&
\\{3,\\{3,\\{3,\\{3,\\{3,3,3[2]\\{3,\\{3,\\{3,\\{3,\\{3,3,3[2]\\{3,\\{\\underbrace{3,\\cdots,3}\_{3\\uparrow\\uparrow\\uparrow3}\\},2[2]2\\}\\}[2]1,2\\},2[2]1,2\\}[2]2,3\\}[2]2,2\\},2\\}[2]1,3\\},2[2]1,3\\}
\\end{eqnarray*}

----

\\begin{eqnarray*} \\{3 \\langle 0 [2]\\backslash 2 \\rangle 2\\} &=& \\{3 \\langle 2 \\backslash 2 \\rangle 2\\} \\\\ &=&
\\{3,3[2]3,3[1 \\backslash 2]3,3[2]3,3[2 \\backslash 2]3,3[2]3,3[1 \\backslash 2]3,3[2]3,3\\}
\\end{eqnarray*}

# Nested Hyper-Nested arrays

This part consists of 2 parts.

## Negations

-   **Rule A1**. $\\textrm\` a \\langle 0 \\neg \\# \\rangle b \\textrm' = \\textrm\` a \\textrm'$.
-   **Rule A2**. If $b = 1$, we have $\\textrm\` a \\langle A \\neg B \\rangle 1 \\textrm' = \\textrm\` a \\textrm'$.
-   **Rule A3**. If $[A] < [B]$, $\\textrm\` a \\langle \\# [A] 1 [B] \\#^* \\neg \\% \\rangle b \\textrm' = \\textrm\` a \\langle \\# [B] \\#^* \\neg \\% \\rangle b \\textrm'$.
-   **Rule A4**. If the first entry in the angle brackets is zero:
-   : $\\textrm\` a \\langle 0 [A\_{1,1}] 1 [A\_{1,2}] \\cdots [A\_{1,p\_1}] c\_1 \\#\_1 \\neg \\#^* \\rangle b \\textrm' = \\textrm\` a \\langle S\_1 \\neg \\#^* \\rangle b \\textrm'$. Set i to 1.
:* *Rule A4a*. $[A\_{i,p\_i}] = [1 \\neg 1 [A\_{i+1,1}] 1 [A\_{i+1,2}] \\cdots [A\_{i+1,p\_{i+1}}] c\_i \\#\_i]$:
::: $S\_i = \\textrm\` b \\langle A\_{i,1}' \\rangle b [A\_{i,1}] b \\langle A\_{i,2}' \\rangle b [A\_{i,2}] \\cdots [A\_{i,p\_i-1}] b \\langle b \\neg S\_{i+1} \\rangle b [A\_{i,p\_i}] c\_i \\#\_i \\textrm'$. Increase i by 1 and follow Rules A4a~d again.
:* *Rule A4b*. $[A\_{i,p\_i}] = \\backslash$:
::: $S\_i = \\textrm\` R\_b \\textrm'$,
::: $R\_n = \\textrm\` b \\langle A\_{i,1}' \\rangle b [A\_{i,1}] b \\langle A\_{i,2}' \\rangle b [A\_{i,2}] \\cdots [A\_{i,p\_i-1}] b \\langle R\_{n-1} \\rangle b [A\_{i,p\_i}] c\_i-1 \\#\_i \\textrm'$,
::: $R\_1 = \\textrm\` 0 \\textrm'$.
    - *Rule A4c*. Rule A4b don't apply, $[A\_{i,p\_i}] = [1 \\neg k \\#\_{i+1}] (k>1)$:
::: $S\_i = \\textrm\` b \\langle A\_{i,1}' \\rangle b [A\_{i,1}] b \\langle A\_{i,2}' \\rangle b [A\_{i,2}] \\cdots [A\_{i,p\_i-1}] b \\langle R\_b \\rangle b [A\_{i,p\_i}] c\_i-1 \\#\_i \\textrm'$,
::: $R\_n = \\textrm\` b \\langle A\_{i,1}' \\rangle b [A\_{i,1}] b \\langle A\_{i,2}' \\rangle b [A\_{i,2}] \\cdots [A\_{i,p\_i-1}] b \\langle R\_{n-1} \\rangle b [A\_{i,p\_i}] c\_i-1 \\#\_i \\neg k-1 \\#\_{i+1} \\textrm'$,
::: $R\_1 = \\textrm\` 0 \\textrm'$.
    - *Rule A4d*. Otherwise:
::: $S\_i = \\textrm\` b \\langle A\_{i,1}' \\rangle b [A\_{i,1}] b \\langle A\_{i,2}' \\rangle b [A\_{i,2}] \\cdots [A\_{i,p\_i-1}] b \\langle A\_{i,p\_i}' \\rangle b [A\_{i,p\_i}] c\_i-1 \\#\_i \\textrm'$.
-   **Rule A5**. Otherwise, $\\textrm\` a \\langle c \\# \\neg \\#^* \\rangle b \\textrm' = \\textrm\` \\underbrace{a \\langle c-1 \\# \\neg \\#^* \\rangle b [c \\#] \\cdots [c \\#] a \\langle c-1 \\# \\neg \\#^* \\rangle b}\_b \\textrm'$.

Note: $\\#, \\#^*, and \\%$ does not contain $\\neg$s.

Limit: $\\{n,n[1[1\\neg1\\neg2]2]2\\}$ has growth rate $\\theta(\\Omega^\\Omega)$.

### Examples

\\begin{eqnarray*} \\{3 \\langle 0 [1 \\neg 1 \\backslash 2] 2 \\rangle 3\\} &=& \\{3 \\langle 3 \\langle 3 \\neg 3,3[2]3,3[3]3,3[2]3,3 \\rangle 3 \\rangle 3\\} \\end{eqnarray*}

----

\\begin{eqnarray*} \\{3 \\langle 0 [1 \\neg 4] 2 \\rangle 3\\} &=& \\{3 \\langle 3 \\langle 3 \\langle 3 \\neg 3 \\rangle 3 \\neg 3 \\rangle 3 \\rangle 3\\} \\end{eqnarray*}

## Hierarchal backslashes

-   **Rule A1**. $\\textrm\` a \\langle 0 \\backslash\_n \\# \\rangle b \\textrm' = \\textrm\` a \\textrm', n>1$.
-   **Rule A2**. If $b = 1$, we have $\\textrm\` a \\langle \\# \\rangle 1 \\textrm' = \\textrm\` a \\textrm'$.
-   **Rule A3**. If $[A] < [B]$, $\\textrm\` a \\langle \\# [A] 1 [B] \\#^* \\rangle b \\textrm' = \\textrm\` a \\langle \\# [B] \\#^* \\neg \\% \\rangle b \\textrm'$.
-   **Rule A4**. If the first entry in the angle brackets is zero:
-   : $\\textrm\` a \\langle 0 [A\_{1,1,1}] 1 [A\_{1,1,2}] \\cdots [A\_{1,1,p\_{1,1}}] c\_{1,1} \\#\_{1,1} \\backslash\_n \\#^* \\rangle b \\textrm' = \\textrm\` a \\langle S\_{1,1} \\backslash\_n \\#^* \\rangle b \\textrm', n>1$. Set i and j to 1.
    - *Rule A4a*. $[A\_{i,1,p\_{i,1}}] = \\backslash$:
::: $S\_{i,1} = \\textrm\` R\_b \\textrm'$,
::: $R\_n = \\textrm\` b \\langle A\_{i,1,1}' \\rangle b [A\_{i,1,1}] b \\langle A\_{i,1,2}' \\rangle b [A\_{i,1,2}] \\cdots [A\_{i,1,p\_{i,1}-1}] b \\langle R\_{n-1} \\rangle b [A\_{i,1,p\_{i,1}}] c\_{i,1}-1 \\#\_{i,1} \\textrm'$,
::: $R\_1 = \\textrm\` 0 \\textrm'$.
    - *Rule A4b*. $[A\_{i,j,p\_{i,1}}] = \\backslash\_j, j>1$:
::: $S\_{i,j} = \\textrm\` R\_{b,j-1} \\textrm'$,
::: $R\_{n,j-1}$
$= \\textrm\` b \\langle A\_{i,j,1}' \\rangle b [A\_{i,j,1}] b \\langle A\_{i,j,2}' \\rangle b [A\_{i,j,2}] \\cdots b \\langle A\_{i,j,p\_{i,j}-1}' \\rangle b [A\_{i,j,p\_{i,j}-1}] b \\langle A\_{i,1,1}' \\rangle b [A\_{i,1,1}] b \\langle A\_{i,1,2}' \\rangle b [A\_{i,1,2}] \\cdots b \\langle A\_{i,1,p\_{i,1}-1}' \\rangle b [A\_{i,1,p\_{i,1}-1}] b \\langle R\_{n-1,1} \\rangle b [A\_{i,1,p\_{i,1}}] c\_{i,1}-1 \\#\_{i,1} \\backslash\_j c\_{i,j}-1 \\#\_{i,j} \\textrm'$,
::: $R\_{n,k} = \\textrm\` b \\langle A\_{i,k+1,1}' \\rangle b [A\_{i,k+1,1}] b \\langle A\_{i,k+1,2}' \\rangle b [A\_{i,k+1,2}] \\cdots b \\langle A\_{i,k+1,p\_{i,k+1}-1}' \\rangle b [A\_{i,k+1,p\_{i,k+1}-1}] b \\langle R\_{n,k+1} \\rangle b [A\_{i,k+1,p\_{i,k+1}}] c\_{i,k+1}-1 \\#\_{i,k+1} \\textrm'$
::: $R\_{1,1} = \\textrm\` 0 \\textrm'$.
    - *Rule A4e*. Otherwise:
::: $S\_i = \\textrm\` b \\langle A\_{i,1,1}' \\rangle b [A\_{i,1,1}] b \\langle A\_{i,1,2}' \\rangle b [A\_{i,1,2}] \\cdots [A\_{i,1,p\_{i,1}-1}] b \\langle A\_{i,1,p\_{i,1}}' \\rangle b [A\_{i,1,p\_{i,1}}] c\_{i,1}-1 \\#\_{i,1} \\textrm'$.
-   **Rule A5**. Otherwise, $\\textrm\` a \\langle c \\# \\rangle b \\textrm' = \\textrm\` \\underbrace{a \\langle c-1 \\# \\rangle b [c \\#] \\cdots [c \\#] a \\langle c-1 \\# \\rangle b}\_b \\textrm'$.

# Hierarchal Hyper-Nested arrays

# Nested Hierarchal Hyper-Nested arrays
